Trying with the original slashed_2

Casper.thy
@@ -10,16 +10,11 @@ locale byz_quorums =
     (* and "\<And> q . \<exists> n . n \<in>\<^sub>2 q" *)
 
 record ('n,'h,'v)state =
-  -- "@{typ 'n} is the type of validators (nodes), @{typ 'h} hashes, and @{typ 'v} views"
-  commit_msg :: "'n \<Rightarrow> 'h \<Rightarrow> 'v \<Rightarrow> bool"
-  prepare_msg :: "'n \<Rightarrow> 'h \<Rightarrow> 'v \<Rightarrow> 'v \<Rightarrow> bool"
+  -- "@{typ 'n} is the type of validators (nodes), @{typ 'h} hashes, and @{typ nat} views"
+  commit_msg :: "'n \<Rightarrow> 'h \<Rightarrow> nat \<Rightarrow> bool"
+  prepare_msg :: "'n \<Rightarrow> 'h \<Rightarrow> nat \<Rightarrow> 'v \<Rightarrow> bool"
 
 locale casper = byz_quorums +
-  views:linorder view_less_eq view_less + 
-  order_bot  bot view_less_eq view_less for
-  view_less_eq :: "'v \<Rightarrow> 'v \<Rightarrow> bool" (infix "\<le>\<^sub>v" 50)
-  and view_less :: "'v \<Rightarrow> 'v \<Rightarrow> bool" (infix "<\<^sub>v" 50)
-  and bot::"'v" ("\<bottom>") +
 fixes 
   hash_pred :: "'h \<Rightarrow> 'h \<Rightarrow> bool" (infix "\<leftarrow>" 50)
 assumes
@@ -31,44 +26,76 @@ begin
 inductive hash_ancestor (infix "\<leftarrow>\<^sup>*" 50) where 
   "h1 \<leftarrow> h2 \<Longrightarrow> h1 \<leftarrow>\<^sup>* h2"
 | "\<lbrakk>h1 \<leftarrow> h2; h2 \<leftarrow>\<^sup>* h3\<rbrakk> \<Longrightarrow> h1 \<leftarrow>\<^sup>* h3"
+declare hash_ancestor.intros[simp,intro]
+
+inductive nth_parent :: "nat \<Rightarrow> 'h \<Rightarrow> 'h \<Rightarrow> bool" where 
+  "nth_parent 0 h1 h1"
+| "\<lbrakk>nth_parent n h1 h2; h2 \<leftarrow> h3\<rbrakk> \<Longrightarrow> nth_parent (n+1) h1 h3"
+declare nth_parent.intros[simp,intro]
+
+inductive_cases test2:"nth_parent 1 h1 h2"
+thm test2
 
 lemmas casper_assms_def = casper_def casper_axioms_def class.linorder_def class.order_def
     class.preorder_def class.order_axioms_def class.linorder_axioms_def byz_quorums_def
     class.order_bot_def class.order_bot_axioms_def
 
-text {* All messages in epoch @{term \<bottom>} are ignored;  @{term \<bottom>} is used as a special value. *}
+text {* All messages in epoch @{term 0} are ignored;  @{term 0} is used as a special value. *}
 
 definition prepared where 
-  "prepared s q h v1 v2 \<equiv> v1 \<noteq> \<bottom> \<and> (\<forall> n . n \<in>\<^sub>1 q \<longrightarrow> prepare_msg s n h v1 v2)"
+  "prepared s q h v1 v2 \<equiv> v1 \<noteq> 0 \<and> (\<forall> n . n \<in>\<^sub>1 q \<longrightarrow> prepare_msg s n h v1 v2)"
 definition committed where
-  "committed s q h v \<equiv> v \<noteq> bot \<and> (\<forall> n . n \<in>\<^sub>1 q \<longrightarrow> commit_msg s n h v)"
+  "committed s q h v \<equiv> v \<noteq> 0 \<and> (\<forall> n . n \<in>\<^sub>1 q \<longrightarrow> commit_msg s n h v)"
 definition fork where 
   "fork s \<equiv> \<exists> h1 h2 q1 q2 v1 v2 . committed s q1 h1 v1 \<and> committed s q2 h2 v2
     \<and> \<not>(h2 \<leftarrow>\<^sup>* h1 \<or> h1 \<leftarrow>\<^sup>* h2 \<or> h1 = h2)"
 
 definition slashed_1 where  "slashed_1 s n \<equiv> 
-  \<exists> h v . commit_msg s n h v \<and> (\<forall> q v2 . v2 <\<^sub>v v \<longrightarrow> \<not>prepared s q h v v2)"
+  \<exists> h v . commit_msg s n h v \<and> (\<forall> q v2 . v2 < v \<longrightarrow> \<not>prepared s q h v v2)"
 definition slashed_2 where
-  -- "this is not exactly what Vitalik wrote."
   "slashed_2 s n \<equiv>
-  \<exists> h v1 v2 . prepare_msg s n h v1 v2 \<and> v2 \<noteq> \<bottom> \<and>
-    (\<forall> v3 q h2 . v3 <\<^sub>v v2 \<longrightarrow> \<not>(h2 \<leftarrow> h \<and> prepared s q h2 v2 v3))"
+  \<exists> h v1 v2 . prepare_msg s n h v1 v2 \<and> v2 \<noteq> 0 \<and>
+    (\<forall> v3 q h2 . v3 < v2 \<longrightarrow> \<not>(nth_parent (v1 - v2) h2 h \<and> prepared s q h2 v2 v3))"
+definition slashed_2' where
+  -- "this is not exactly what Vitalik wrote."
+  "slashed_2' s n \<equiv>
+  \<exists> h v1 v2 . prepare_msg s n h v1 v2 \<and> v2 \<noteq> 0 \<and>
+    (\<forall> v3 q h2 . v3 < v2 \<longrightarrow> \<not>(h2 \<leftarrow> h \<and> prepared s q h2 v2 v3))"
 definition slashed_3 where 
   "slashed_3 s n \<equiv>
-  \<exists> h1 h2 v1 v2 v3 . v1 <\<^sub>v v2 \<and> v3 <\<^sub>v v1 \<and> 
+  \<exists> h1 h2 v1 v2 v3 . v1 < v2 \<and> v3 < v1 \<and> 
     commit_msg s n h1 v1 \<and> prepare_msg s n h2 v2 v3"
 definition slashed_4 where
   "slashed_4 s n \<equiv> \<exists> h1 h2 v v1 v2 . (h1 \<noteq> h2 \<or> v1 \<noteq> v2) \<and> 
     prepare_msg s n h1 v v1 \<and> prepare_msg s n h2 v v2"
 
 definition slashed where "slashed s n \<equiv> 
-  slashed_1 s n \<or> slashed_2 s n \<or> slashed_3 s n \<or>  slashed_4 s n"
+  slashed_1 s n \<or> slashed_2 s n \<or> slashed_3 s n \<or> slashed_4 s n"
+
+lemma assumes "prepared s q h1 v1 v2" and "committed s q h2 v2" and "v1 > v2"
+  and "\<not>nth_parent (v1 - v2) h2 h1"
+shows "\<exists> q . \<forall> n . n \<in>\<^sub>2 q \<longrightarrow> slashed s n"
+  using assms
+proof (induct "v1 - v2 - 1")
+  case 0
+  have "\<not>h2 \<leftarrow> h1"
+    by (metis "0.hyps" Nat.add_0_right One_nat_def Suc_diff_Suc add_Suc_right assms(3) assms(4) diff_diff_left nth_parent.intros(1) nth_parent.intros(2))  
+  then show ?case using 0
+  using assms casper_axioms nth_parent.intros
+  unfolding slashed_def slashed_1_def slashed_2_def slashed_4_def slashed_3_def
+      prepared_def fork_def committed_def casper_assms_def
+  apply auto
+  using [[smt_infer_triggers,smt_timeout=3000,smt_oracle=true,smt_random_seed=3143,smt_certificates="./casper.cert"]]
+next
+  case (Suc x)
+  then show ?case sorry
+qed oops
 
 lemma assumes "fork s"
-  shows "\<exists> q . \<forall> n . n \<in>\<^sub>2 q \<longrightarrow> slashed s n"
+  shows "\<exists> q . \<forall> n . n \<in>\<^sub>2 q \<longrightarrow> slashed s n" oops
   using [[]]
-  nitpick[verbose, card 'b=2, card 'c=2, card 'a=5, card 'v=4, card 'h=3, card 'd=1,
-      card "('a, 'h, 'v, 'd) state_scheme" = 1, dont_box, timeout=300] (*,
+  nitpick[verbose, card 'b=2, card 'c=2, card 'a=5, card nat=5, card 'h=4, card 'd=1,
+      card "('a, 'h, nat, 'd) state_scheme" = 1, dont_box, timeout=300] (*,
       eval="(slashed s, committed s)"] *)
   using assms casper_axioms
   apply -
@@ -76,11 +103,11 @@ lemma assumes "fork s"
       prepared_def fork_def committed_def
   apply (cases s)
   apply simp
-  using hash_ancestor.intros
+  using hash_ancestor.intros nth_parent.intros
   unfolding casper_assms_def
   apply (simp (no_asm_use))
   apply (match premises in P[thin]:"?x = ?y" \<Rightarrow> \<open>-\<close>)
-  apply clarify
+  apply clarify oops
   using [[smt_infer_triggers,smt_timeout=3000,smt_oracle=true,smt_random_seed=8789797972,smt_certificates="./casper.cert"]]
   sledgehammer[timeout=5000, provers=z3 spass]()
 
